tuesday

PolyComPed.ec
@@ -219,7 +219,10 @@ clone export PolynomialCommitment as PolyComPed with
 
   lemma PolyComDL2_Corr :
   hoare[Correctness(PolyCommitPed).main : true ==> res].
-  proof.
+      proof.
+        admit.
+      (*
+     
      proc. inline*. auto. progress. case (Bl.t{hr} < deg p{hr}). smt(). move => h'.
     simplify. 
     (* Lift everything to exp *)
@@ -266,12 +269,12 @@ clone export PolynomialCommitment as PolyComPed with
     have : forall (a b c : exp), a * (b + c) = (a * b) + (a * c).
   move => ? ? ?. rewrite ZModpField.mulrC. rewrite ZModpField.mulrDl.
   smt(@ZModpField). move => g'. rewrite g'.
-    smt(@Bl.GP).
+    smt(@Bl.GP).*)
 qed.
 
 axiom expg_modz_gen (b : Bl.GB.group) k : b ^ (k %% Bl.GB.order) = b ^ k.
 
-axiom expe (b :  Bl.GB.group) : Bl.GPB.loge b <> Bl.GPB.ZModE.zero <=> b <> Bl.GB.e.
+axiom expe (b :  Bl.GB.group) : Bl.ZP.loge b <> Bl.ZP.ZModE.zero <=> b <> Bl.GB.e.
 
 op isValid (k : (Bl.GB.group * Bl.GB.group) list)  =
   all (fun (y : Bl.GB.group) => y <> Bl.GB.e) (unzip2 k).
@@ -283,31 +286,40 @@ op isValid (k : (Bl.GB.group * Bl.GB.group) list)  =
     factorFind (p - p')
   (map (fun (i : int) => Bl.GB.g ^ asint (exp a i))
      (range 0 (Bl.t + 1))) = a.
-
+(*fixed*)
    lemma not_inv (x : exp) : one - x <> - x.
        have : forall (a b c : exp), a <> c + b => a - b <> c.
-       smt(@Bl.GP.ZModE). move => h. apply h. smt(@Bl.GP.ZModE).
+       smt(@Bl.ZP.ZModE). move => h. apply h. smt(@Bl.ZP.ZModE).
      qed.
 
   section Security.
 
   declare module A_PB <: AdvPB {-PolyCommitPed.bad}.
+
+(*fixed*)
+  module Adv (A : AdvPB) : Bl.TsdhAdv2 = {
+  proc comp(h : (Bl.GB.group * Bl.GB.group) list) : (exp -> exp) * (exp -> Bl.GB.group) = {
+    var c, phi, phi', d, d';
+        (c, phi, phi', d, d') <@ A.forge(unzip1 h, unzip2 h);
     
-  module Adv  : Bl.TsdhAdv2 = {
-    proc comp(h : (Bl.GB.group * Bl.GB.group) list) : (exp -> exp) * (exp -> Bl.GB.group) = {
-      var c, phi, phi', d, d';
-      (c, phi, phi', d, d') <@ A_PB.forge(unzip1 h, unzip2 h);
-      return (if (prodEx Bl.GB.g (unzip1 h) phi = prodEx Bl.GB.g (unzip1 h) phi') then
-        ((fun e => one - factorFind (phi - phi') (unzip1 h)), (fun e=>Bl.GB.g))
-      else
-       ((fun (e : exp)  => (peval phi' e - peval phi e) / (peval d e - peval d' e)), (fun e => Bl.GB.g)));
-    }
-  }.
+    return (if (prodEx Bl.GB.g (unzip1 h) phi = prodEx Bl.GB.g (unzip1 h) phi') then
+      ((fun e => one - factorFind (phi - phi') (unzip1 h)), (fun e=>Bl.GB.g))
+    else
+      ((fun (e : exp) => (peval phi' e - peval phi e) / (peval d e - peval d' e)), (fun e => Bl.GB.g)));
+  }
+}.
+
+
+ 
+ 
   
-  lemma PolyComDLScheme_PolynomialBinding &m  :
-        Pr[PolynomialBinding(PolyCommitPed, A_PB).main() @ &m : res]  <=
-        Pr[Bl.Tsdh2(Adv).main() @ &m :res].
-  proof. 
+  
+ lemma PolyComDLScheme_PolynomialBinding &m :
+  Pr[PolynomialBinding(PolyCommitPed, A_PB).main() @ &m : res] <=
+  Pr[Bl.Tsdh2(Adv(A_PB)).main() @ &m : res].
+  proof.
+  admit.
+  (*
     byequiv. proc. inline *. auto. call (_ : true). auto. progress.
     (* key valid *)
     rewrite unzip1_zip. smt(@List). trivial. rewrite unzip2_zip. smt(@List). trivial.
@@ -330,29 +342,47 @@ op isValid (k : (Bl.GB.group * Bl.GB.group) list)  =
 
     smt(@Bl.GP.ZModE). move => h''''. apply h'''' in H9. smt(@Bl.GP.ZModE).
     (* Misc *)
-    smt(). smt(). 
+    smt(). smt(). *)
   qed.
 
   declare module A_EB <: AdvEB {-PolyCommitPed.bad}.
-  
-  module Adv2 : Bl.TsdhAdv2 = {
-    proc comp(h : (Bl.GB.group * Bl.GB.group) list) : (exp ->  exp) * (exp -> Bl.GB.group)  = {
-      var c, i, phi, phi', d, d';
-      (c, i, phi, d, phi', d') <@ A_EB.forge(unzip1 h, unzip2 h);
-      return (if (d.`2 <> d'.`2) then
-        if (Bl.GB.g^(asint i) = nth Bl.GB.g (unzip1 h) 1) then
-        ((fun e => one - i), (fun e => Bl.GB.g)) else 
-        ((fun e => -i), (fun e => (Bl.GB.( / ) d.`2 d'.`2)^(asint (one/(phi' + e*d'.`1-(phi+e*d.`1))))))
+
+
+
+
+(*fixed*)
+module Adv2 (A : AdvEB) : Bl.TsdhAdv2 = {
+  proc comp(h : (Bl.GB.group * Bl.GB.group) list) : (exp -> exp) * (exp -> Bl.GB.group) = {
+    var c, i, phii, w, phii', w';
+    
+    (c, i, phii, w, phii', w') <@ A.forge(unzip1 h, unzip2 h);
+    
+    return (if (w.`2 <> w'.`2) then
+        if (Bl.ZP.( ^ ) Bl.GB.g i = nth Bl.GB.g (unzip1 h) 1) then
+          ((fun (e : exp) => one - i), (fun (e : exp) => Bl.GB.g)) 
+        else 
+          ((fun (e : exp) => -i), 
+           (fun (e : exp) => 
+              let base = Bl.GB.( * ) w.`2 (Bl.GB.inv w'.`2) in
+              let p_exp = inv (phii' + e * w'.`1 - (phii + e * w.`1)) in
+              Bl.ZP.( ^ ) base p_exp))
       else
-       ((fun e => (phi' - phi) / (d.`1 - d'.`1)),(fun e=> Bl.GB.g)));
-    }
-  }.
+        ((fun (e : exp) => (phii' - phii) / (w.`1 - w'.`1)), (fun (e : exp) => Bl.GB.g)));
+  }
+}.
+  
+
+
 
   
-  lemma PolyDL2_eval_sound &m :
-      Pr[EvaluationBinding(PolyCommitPed, A_EB).main() @ &m :res] <=
-      Pr[Bl.Tsdh2(Adv2).main() @ &m : res].
-   proof.   
+
+  
+ lemma PolyDL2_eval_sound &m :
+  Pr[EvaluationBinding(PolyCommitPed, A_EB).main() @ &m : res] <=
+  Pr[Bl.Tsdh2(Adv2(A_EB)).main() @ &m : res].
+  proof.
+  admit.
+  (*
      byequiv. proc. inline*. auto. call(:true). auto. progress.
      (* key valid *)
     rewrite unzip1_zip. smt(@List). trivial. rewrite unzip2_zip. smt(@List). trivial.
@@ -402,9 +432,10 @@ op isValid (k : (Bl.GB.group * Bl.GB.group) list)  =
      rewrite !inzmodD in h'. rewrite !inzmodM in h'.  rewrite !asintK in h'. rewrite !Bl.GP.ZModE.ZModpField.mulr1 in h'.
      apply Bl.exp_a_bc. smt(@ZModpField). trivial.
     (* nonsense *)
-    smt(). smt().
+    smt(). smt().*)
    qed.
 
+   (*fixed*)
  module HidingSimp (A : AdvH) = {
 
   var bad : bool
@@ -435,7 +466,7 @@ op isValid (k : (Bl.GB.group * Bl.GB.group) list)  =
      js <@ A.choose(key, c);
          phi <$ dpoly Bl.t Bl.FD.dt;
      d <- ((inv b) ** (m1  - phi));
-     phiis <- map  (fun (x1 : Bl.GP.exp) => peval phi x1) js;
+     phiis <- map  (fun (x1 : Bl.ZP.exp) => peval phi x1) js;
        ws <- [];                                                      
        j <- 0;                                             
        while (j < Bl.t - 1) {                                                                 
@@ -561,24 +592,27 @@ op isValid (k : (Bl.GB.group * Bl.GB.group) list)  =
 
      declare module A_H <: AdvH {-PolyCommitPed.bad, -HidingSimp.bad}.
 
-  lemma count_not_x x : count (fun (x0 : Bl.GP.exp) => x0 <> x) (map inzmod (range 0 Bl.GT.order)) = Bl.GT.order -1.
-  proof.
-    have : uniq (map inzmod (range 0 Bl.GT.order)). smt(@List @Bl.GP.ZModE). move => h.
-    have : Bl.GT.order = size  (map inzmod (range 0 Bl.GT.order)). smt(@List). move => h'. rewrite h'.
+  lemma count_not_x x : count (fun (x0 : Bl.ZP.exp) => x0 <> x) (map inzmod (range 0 Bl.GT.order)) = Bl.GT.order -1.
+      proof.
+      
+    have : uniq (map inzmod (range 0 Bl.GT.order)). smt(@List @Bl.ZP.ZModE). move => h.
+    have : Bl.GT.order = size  (map inzmod (range 0 Bl.GT.order)). smt(@List prime_p). move => h'. rewrite h'.
     rewrite countC. rewrite !size_map. rewrite !size_range. rewrite count_uniq_mem. smt(@Bl.GT).
-    smt(@Bl.GP.ZModE).
+    smt(@Bl.ZP.ZModE).
   qed.
 
   lemma mu_FD js : size js = Bl.t - 1 =>
-  0%r < mu Bl.FD.dt (fun (x : Bl.GP.exp) => ! (x \in js)).
-  proof. 
-    move => h. apply (AddDistr.mu_list _ _ Bl.GT.order). rewrite Bl.GP.ZModE.DZmodP.dunifinE.
+  0%r < mu Bl.FD.dt (fun (x : Bl.ZP.exp) => ! (x \in js)).
+      proof.
+        
+      
+    move => h. apply (AddDistr.mu_list _ _ Bl.GT.order). rewrite Bl.ZP.ZModE.DZmodP.dunifinE.
     have : forall (a a' b b' : real), a <= a' => b = b' => 0%r < b => a / b <= a' / b'.
     move => a a' b b' h' h'' h'''. subst. elim h' => h'. left. smt(). smt(). move => h'. apply h'.
     move => @/DZmodP.Support.enum. clear h. elim js. smt(@List). move => x l ind_hyp. simplify.
     case (x \in l). smt(@List). move => g. have : (fun (x0 : exp) => ! (x0 = x \/ (x0 \in l))) =
     predI (fun x0 => x0 <> x)(fun x0 => (! x0 \in l)). smt(). move => h. rewrite h.
-    rewrite countI. rewrite count_not_x. smt(@List). smt(@Bl.GP.ZModE). smt(@Bl.GT). smt(Bl.t_lt_card).
+    rewrite countI. rewrite count_not_x. smt(@List prime_p). smt(@Bl.ZP.ZModE). smt(@Bl.GT). smt(Bl.t_lt_card).*)
   qed.
 
 (* The adversary cannot do better then randomly guessing an evaulation point *)
@@ -586,7 +620,9 @@ op isValid (k : (Bl.GB.group * Bl.GB.group) list)  =
      islossless A_H.choose =>
      islossless A_H.guess =>   
   Pr[HidingSimp(A_H).rand() @ &m : res] <= (1%r/ Bl.GB.order%r).
-proof.
+  proof.
+    admit.
+    (*
   move => Ac_ll Ah_ll. byphoare. proc. inline *. seq 8 : true 1%r (1%r / Bl.GB.order%r) 0%r _ true. auto.
   conseq (_ : _ ==> _ : =1%r). call(_:true). auto. progress. smt(@Bl.FD). apply dpoly_ll. smt(@Bl.FD).
   if. swap [1..2] 5.  seq 5 : (size js = Bl.t - 1) 1%r (1%r / Bl.GB.order%r) 0%r _ true. auto. auto.
@@ -598,7 +634,7 @@ proof.
   apply interpolate_prob2_dcond; trivial.
   (* js size flips *)
   conseq (_ : _ ==> _ : =0%r). auto. hoare. call(_:true). while (size js = Bl.t-1).  auto. progress. auto. progress.
-  conseq (_ : _ ==> _ : =0%r). smt(@Bl.GB). hoare. auto. progress. smt(). auto. smt(). trivial. trivial.
+  conseq (_ : _ ==> _ : =0%r). smt(@Bl.GB). hoare. auto. progress. smt(). auto. smt(). trivial. trivial.*)
 qed.
 
 lemma HidingSimp_Flip &m :
@@ -613,11 +649,26 @@ proof.
   auto. auto. auto.
 qed.
 
+
+
+
+
+
+
+    (*got up to here need to change the asintmul*)
+
+
+
+
+
 lemma Hiding_comm_sim  &m :
     islossless A_H.guess =>
     islossless A_H.choose =>
     Pr[Hiding(PolyCommitPed,A_H).real() @ &m : res] <=  Pr[HidingSimp(A_H).comm_sim() @ &m : res  \/ HidingSimp.bad].
-proof.
+    proof.
+admit.
+
+    (*
   move => Ag_ll Ac_ll. byequiv. proc. inline *. swap{1} [4..5] -3. swap{2} [3..4] -2. seq 1 1 : (={glob A_H, b}).
   rnd. auto. progress.
 
@@ -631,34 +682,53 @@ proof.
   (* resuming main *)
   call(_:true). while(={j,js,ws,key,phi,d}). auto. progress.
   swap{2} 9 -8. wp. call(_:true). wp.  rnd(fun m1 => phi{1} + (b{2} ** m1))(fun m1 => (inv b{2}) ** (m1-phi{1})). auto. 
-  progress. smt(). smt(). smt(). smt(). smt().  rewrite scalepA. rewrite  Bl.GP.ZModE.ZModpRing.divrr.
-  apply Bl.GP.ZModE.unitE; trivial. rewrite scale_1; trivial. smt(@IDPoly). rewrite size_mkseq.
+  progress. smt(). smt(). smt(). smt(). smt().  rewrite scalepA. rewrite  Bl.ZP.ZModE.ZModpRing.divrr.
+  apply Bl.ZP.ZModE.unitE; trivial. rewrite scale_1; trivial. smt(@IDPoly). rewrite size_mkseq.
   have: (max 0 (Bl.t + 1) - 1) = Bl.t. smt(Bl.t_valid). move => h. rewrite h. apply dpoly_uni. smt(Bl.t_valid). smt(@Bl.FD).
   apply dpoly_fu. smt(Bl.t_valid). smt(@Bl.FD). rewrite supp_dpoly in H5.  smt(Bl.t_valid). smt(@Bl.FD).
   apply dpoly_fu. smt(Bl.t_valid). smt(@Bl.FD). apply degZ_le_gen. apply degD_sim.  rewrite supp_dpoly in H5.  smt(Bl.t_valid). 
   smt().  rewrite supp_dpoly in H0.  smt(Bl.t_valid). smt(degN).  apply dpoly_fu. smt(Bl.t_valid). smt(@Bl.FD). apply degD_sim.
   rewrite supp_dpoly in H0.  smt(Bl.t_valid). smt(degN). apply degZ_le_gen. rewrite size_mkseq in H6. rewrite supp_dpoly in H6.
   smt(Bl.t_valid). smt(Bl.t_valid). have : phiL + b{2} ** m1L - phiL = b{2} ** m1L. smt(@IDPoly). move => h. rewrite h.
-  rewrite scalepA. rewrite Bl.GP.ZModE.ZModpRing.mulrC. rewrite Bl.GP.ZModE.ZModpRing.divrr. apply Bl.GP.ZModE.unitE; trivial.
+  rewrite scalepA. rewrite Bl.ZP.ZModE.ZModpRing.mulrC. rewrite Bl.ZP.ZModE.ZModpRing.divrr. apply Bl.ZP.ZModE.unitE; trivial.
   rewrite scale_1; trivial. rewrite !head_mkKey !comPolEval.  rewrite supp_dpoly in H0.  smt(Bl.t_valid). smt(@Bl.FD).
   rewrite size_mkseq in H6. rewrite supp_dpoly in H6.  smt(Bl.t_valid). smt(Bl.t_valid). apply degD_sim.
   rewrite supp_dpoly in H0.  smt(Bl.t_valid). smt(). apply degZ_le_gen. rewrite size_mkseq in H6. rewrite supp_dpoly in H6.
-  smt(Bl.t_valid). smt(Bl.t_valid). rewrite -Bl.GB.expM. rewrite Bl.exp_GB_asint_mul. rewrite -Bl.GB.expD.
-  rewrite Bl.exp_GB_asint_add. rewrite -peval_add. rewrite -peval_mul. smt(@Bl.GP.ZModE).
-  trivial. trivial. 
+  smt(Bl.t_valid). smt(Bl.t_valid). 
+
+  admit.
+
+  rewrite -ZP.pow_pow.
+  rewrite -ZP.pow_add.
+  rewrite -peval_add. 
+  rewrite -peval_mul. 
+  smt(@Bl.ZP.ZModE).
+  
+  trivial. trivial. *)
 qed.
+
+
+
+
+
+
+
 
 lemma dProd_size phiis :  phiis \in Bl.FD.dt `*` dlist Bl.FD.dt (Bl.t - 1) =>
     size phiis.`2 = Bl.t - 1.
-proof.
-  move => h. have : phiis.`2 \in  dlist Bl.FD.dt (Bl.t - 1). smt(@Distr). move => g. smt(@DList Bl.t_valid).
+    proof.
+    admit.
+    (* last smt is failing
+  move => h. have : phiis.`2 \in  dlist Bl.FD.dt (Bl.t - 1). smt(@Distr). move => g. smt(@DList Bl.t_valid).*)
 qed.
     
 lemma Hiding_equiv &m :
     islossless A_H.guess =>
     islossless A_H.choose =>
      Pr[HidingSimp(A_H).comm_sim() @ &m : res \/ HidingSimp.bad] = Pr[HidingSimp(A_H).real() @ &m : res \/ HidingSimp.bad].
-proof.
+     proof.
+       admit.
+       (*
   move => Ag_ll Ac_ll. byequiv (_ : ={glob A_H} ==> (={res,HidingSimp.bad}) \/ (={HidingSimp.bad} /\ HidingSimp.bad{1})).
   proc. inline *. swap{1} [3..4] -2. swap{2} [3..4] -2. seq 1 1 : (={glob A_H, b}).
   rnd. auto. progress. 
@@ -732,8 +802,14 @@ proof.
   (* third stupid case *)
   auto. call{1} (: true ==> true). 
   while{1} (j{1} <= Bl.t -1) (Bl.t-j{1}-1). auto. progress. smt(). smt(). auto. progress. apply dpoly_ll.
-  smt(@Bl.FD). smt(Bl.t_valid). smt(). smt(). trivial. smt().
+  smt(@Bl.FD). smt(Bl.t_valid). smt(). smt(). trivial. smt().*)
 qed.
+
+search Bl.GB.order.
+
+
+
+
 
 
 lemma HidingSimp_real_split &m :
@@ -745,21 +821,25 @@ lemma HidingSimp_real_split &m :
     auto. progress. smt(). smt(). smt(). smt(). auto.
   qed.
 
+ 
 lemma HidingSimp_real_bad &m :
    islossless A_H.choose =>
    islossless A_H.guess => 
    Pr[HidingSimp(A_H).real() @ &m : HidingSimp.bad] + 1%r / Bl.GB.order%r = 2%r / Bl.GB.order%r.
-proof.
+   proof.
+
+     admit.
+   (*
   move => Ac_ll Ag_ll. have :Pr[HidingSimp(A_H).real() @ &m : HidingSimp.bad] = 1%r / Bl.GB.order%r =>
 Pr[HidingSimp(A_H).real() @ &m : HidingSimp.bad] + 1%r / Bl.GB.order%r = 2%r / Bl.GB.order%r. smt().
   move => h. apply h. byphoare. proc.  seq 4 : HidingSimp.bad (1%r / Bl.GB.order%r) 1%r (1%r - (1%r / Bl.GB.order%r)) 0%r true;
-  trivial. wp. rnd. wp. rnd. auto. progress. rewrite Bl.FD.dt1E. smt(Bl.order_eq). smt(@Bl.FD). seq 5 : HidingSimp.bad.
+  trivial. wp. rnd. wp. rnd. auto. progress. rewrite Bl.FD.dt1E. smt(Bl.GB.order_p). smt(@Bl.FD). seq 5 : HidingSimp.bad.
   auto. call( : HidingSimp.bad). auto.  progress. apply dpoly_ll. smt(@Bl). if.  call( : HidingSimp.bad).
   while ( HidingSimp.bad)(Bl.t-1-j). auto. progress. smt(). auto. progress. apply dcond_ll. apply mu_FD; trivial. apply dprod_ll.
   smt(@Bl @DList). smt(). auto. progress. 
   (* the failure event is not negated *)
   hoare. call( : HidingSimp.bad). auto. progress. hoare. seq 5 : (!HidingSimp.bad). call(_:true). auto. if.
-  call(_:true). while (!HidingSimp.bad). auto. progress. auto. auto. trivial. trivial.
+  call(_:true). while (!HidingSimp.bad). auto. progress. auto. auto. trivial. trivial.*)
 qed.
 
 lemma PolyComDL2_Hiding  &m :
@@ -838,18 +918,29 @@ proof.
   move => hi h_all. have: key_valid g ga x i. smt(@List). move => h'. rewrite h'. trivial.
 qed.
 
+
+
+
+
+
+
+
+
+
 lemma nth_from_all_key_valid_ind i g j x:
     g <> Bl.GB.e =>
     all (key_valid g (g^j) x) (range 0 Bl.t) =>
     0 <= i < Bl.t =>
     nth Bl.GB.g x i = g ^ asint (exp (inzmod j) i) =>
     nth Bl.GB.g x (i+1) = g ^ asint (exp (inzmod j) (i+1)).
-proof.
+    proof.
+      admit.
+    (*
   move => g_neq_e h_all hi h_ind. have: key_valid g (g^j) x i. smt(@List). move => @/key_valid. move => h'.
   rewrite h_ind in h'. rewrite Bl.e_pow1 in h'. rewrite -Bl.e_pow2 in h'.
   have : nth Bl.GB.g x (i + 1) = g ^ asint (exp (inzmod j) i) ^ j. apply (Bl.e_inj1 _ _ g); trivial. smt(@Bl).
 move => h. rewrite h. rewrite !exp_inzmod. elim hi => hi hi'. rewrite hi. have : 0 <= i + 1. smt(). move => hii. rewrite hii.
-  simplify. rewrite !inzmodK. rewrite -Bl.order_eq. rewrite !Bl.exp_g_modz. rewrite -Bl.GB.expM. rewrite exprS. smt(). smt().
+  simplify. rewrite !inzmodK. rewrite -Bl.order_eq. rewrite !Bl.exp_g_modz. rewrite -Bl.GB.expM. rewrite exprS. smt(). smt().*)
 qed.
 
 (* resuming *)
@@ -868,7 +959,9 @@ lemma valid_key_extract_corr (key : (Bl.GB.group) list * (Bl.GB.group) list) i j
   all (key_valid Bl.GB.g (nth Bl.GB.g key.`1 1) key.`2) (range 0 Bl.t) =>
     
   key = (mkKey Bl.GB.g (inzmod j), mkKey (Bl.GB.g ^ asint (inzmod i)) (inzmod j)).
-proof.
+    proof.
+      admit.
+    (*
   move => hi hj sk1 sk2 ga_neq0 ha_neq0 all1 all2. rewrite hj in all1. rewrite hj in all2. rewrite pairS. apply pw_eq.
 
   (* left half of key correct *)
@@ -895,7 +988,7 @@ proof.
   simplify. rewrite -!Bl.GB.expM. rewrite !(mulrC (asint (inzmod i))). rewrite !Bl.GB.expM. congr.
   rewrite !inzmodK. rewrite -Bl.order_eq. rewrite !Bl.exp_g_modz. rewrite exprS. smt(). rewrite Bl.GB.expM. smt(@Bl.GB).
   (* Case where i0 is beyond the list *)
-  rewrite !nth_default. smt(). rewrite size_mkseq. smt(Bl.t_valid). trivial.
+  rewrite !nth_default. smt(). rewrite size_mkseq. smt(Bl.t_valid). trivial.*)
 qed.
 
 module Setup_valid_key = {
@@ -909,7 +1002,8 @@ module Setup_valid_key = {
 
 lemma PolyCom_Setup_correct &m :
   Pr[Setup_valid_key.main() @ &m : res] = (1%r - (1%r / Bl.GB.order%r)) ^ 2.
-proof.
+  proof.
+  admit. (*
   byphoare. proc. inline *. swap 2 1.
   seq 2 : (b0 <> zero /\ a <>  zero) ((1%r- (1%r / Bl.GB.order%r))^2) 1%r (1%r- (1%r- (1%r / Bl.GB.order%r))^2)  0%r true; trivial.
   seq 1 : (a <> zero) (1%r- (1%r / Bl.GB.order%r)) (1%r-(1%r/Bl.GB.order%r)) ((1%r / Bl.GB.order%r)^2)  0%r true; trivial.
@@ -935,7 +1029,7 @@ proof.
   rewrite nth_mkseq. smt(Bl.t_valid). simplify. smt(@Bl). 
   rewrite head_mkKey. smt(@Bl).
   (* dumb parts *)
-  hoare. auto. progress. rewrite head_mkKey.  rewrite nth_mkseq. smt(Bl.t_valid). simplify. smt(@Bl). trivial. trivial.
+  hoare. auto. progress. rewrite head_mkKey.  rewrite nth_mkseq. smt(Bl.t_valid). simplify. smt(@Bl). trivial. trivial.*)
  qed.
  
 
@@ -964,7 +1058,7 @@ proof.
      js <@ A.choose(c);
          phi <$ dpoly Bl.t Bl.FD.dt;
      d <- ((inv b) ** (m1  - phi));
-     phiis <- map  (fun (x1 : Bl.GP.exp) => peval phi x1) js;
+     phiis <- map  (fun (x1 : Bl.ZP.exp) => peval phi x1) js;
        ws <- [];                                                      
        j <- 0;                                             
        while (j < Bl.t - 1) {                                                                 
@@ -1089,7 +1183,9 @@ lemma Hiding_BoundS &m :
     islossless A_SH.choose =>
      islossless A_SH.guess =>
     Pr[HidingSimpS(A_SH).rand() @ &m : res] <= (1%r/ Bl.GB.order%r).
-proof.
+    proof.
+      admit.
+    (*
   move => As_ll Ac_ll Ag_ll. byphoare. proc. inline *. seq 15 : true 1%r (1%r / Bl.GB.order%r) 0%r _ true. auto.
   conseq (_ : _ ==> _ : =1%r). call(_:true). auto. while (true)(Bl.GB.order-j0). progress. auto. progress. smt().
   wp. while (true)(Bl.GB.order-i0). progress. auto. progress. smt(). auto. call(_:true). auto. progress. smt(). smt().
@@ -1104,7 +1200,7 @@ proof.
   apply interpolate_prob2_dcond; trivial.
   (* js size flips *)
   conseq (_ : _ ==> _ : =0%r). auto. hoare. call(_:true). while (size js = Bl.t-1).  auto. progress. auto. progress.
-  conseq (_ : _ ==> _ : =0%r). smt(@Bl.GB). hoare. auto. progress. smt(). auto. smt(). trivial. trivial.
+  conseq (_ : _ ==> _ : =0%r). smt(@Bl.GB). hoare. auto. progress. smt(). auto. smt(). trivial. trivial.*)
 qed.
 
 lemma HidingSimp_FlipS &m :
@@ -1129,7 +1225,9 @@ lemma SHiding_equiv1 &m :
     islossless A_SH.choose =>
     islossless A_SH.guess =>
      Pr[Strong_Hiding(PolyCommitPed,PolyCommitPed_A,A_SH).real() @ &m : res] <= Pr[HidingSimpS(A_SH).comm_sim() @ &m : res].
-proof.
+     proof.
+       admit.
+     (*
   move => As_ll Ac_ll Ag_ll. byequiv. proc. swap{1} 1 2. seq 1 1 : (={glob A_SH, key}). call (_:true). auto.
 
   (* discharge case of invalid key *)
@@ -1182,21 +1280,21 @@ proof.
   (* resuming main *)
   call(_:true). inline *.  while(={j,js,ws,key,phi,d}). auto. progress. wp. swap{2} 4 -3. call(_:true). wp.
   rnd(fun m1 => phi{1} + (b{2} ** m1))(fun m1 => (inv b{2}) ** (m1-phi{1})). auto. 
-  progress. rewrite scalepA. rewrite  Bl.GP.ZModE.ZModpRing.divrr.
-  apply Bl.GP.ZModE.unitE; trivial. rewrite scale_1; trivial. smt(@IDPoly). rewrite size_mkseq.
+  progress. rewrite scalepA. rewrite  Bl.ZP.ZModE.ZModpRing.divrr.
+  apply Bl.ZP.ZModE.unitE; trivial. rewrite scale_1; trivial. smt(@IDPoly). rewrite size_mkseq.
   have: (max 0 (Bl.t + 1) - 1) = Bl.t. smt(Bl.t_valid). move => h. rewrite h. apply dpoly_uni. smt(Bl.t_valid). smt(@Bl.FD).
   apply dpoly_fu. smt(Bl.t_valid). smt(@Bl.FD). rewrite supp_dpoly in H3.  smt(Bl.t_valid). smt(@Bl.FD).
   apply dpoly_fu. smt(Bl.t_valid). smt(@Bl.FD). apply degZ_le_gen. apply degD_sim.  rewrite supp_dpoly in H3.  smt(Bl.t_valid). 
   smt().  rewrite supp_dpoly in H0.  smt(Bl.t_valid). smt(degN).  apply dpoly_fu. smt(Bl.t_valid). smt(@Bl.FD). apply degD_sim.
   rewrite supp_dpoly in H0.  smt(Bl.t_valid). smt(degN). apply degZ_le_gen. rewrite size_mkseq in H4. rewrite supp_dpoly in H4.
   smt(Bl.t_valid). smt(Bl.t_valid). have : phiL + b{2} ** m1L - phiL = b{2} ** m1L. smt(@IDPoly). move => h. rewrite h.
-  rewrite scalepA. rewrite Bl.GP.ZModE.ZModpRing.mulrC. rewrite Bl.GP.ZModE.ZModpRing.divrr. apply Bl.GP.ZModE.unitE; trivial.
+  rewrite scalepA. rewrite Bl.ZP.ZModE.ZModpRing.mulrC. rewrite Bl.ZP.ZModE.ZModpRing.divrr. apply Bl.ZP.ZModE.unitE; trivial.
   rewrite scale_1; trivial. rewrite !head_mkKey !comPolEval.  rewrite supp_dpoly in H0.  smt(Bl.t_valid). smt(@Bl.FD).
   rewrite size_mkseq in H4. rewrite supp_dpoly in H4.  smt(Bl.t_valid). smt(Bl.t_valid). apply degD_sim.
   rewrite supp_dpoly in H0.  smt(Bl.t_valid). smt(). apply degZ_le_gen. rewrite size_mkseq in H4. rewrite supp_dpoly in H4.
   smt(Bl.t_valid). smt(Bl.t_valid). rewrite -Bl.GB.expM. rewrite Bl.exp_GB_asint_mul. rewrite -Bl.GB.expD.
   rewrite Bl.exp_GB_asint_add. rewrite -peval_add. rewrite -peval_mul. smt(@Bl.GP.ZModE).
-  trivial. trivial. 
+  trivial. trivial. *)
 qed.     
 
 
@@ -1205,7 +1303,9 @@ lemma SHiding_equiv2 &m :
     islossless A_SH.choose =>
     islossless A_SH.guess =>
     Pr[HidingSimpS(A_SH).real() @ &m : res] = Pr[HidingSimpS(A_SH).comm_sim()  @ &m : res].
-proof.
+    proof.
+      admit.
+    (*
   move => As_ll Ac_ll Ag_ll. byequiv. proc.
 
   seq 1 1 : (={glob A_SH, key}). call(_ : true). auto. progress.
@@ -1320,7 +1420,7 @@ proof.
 
    auto. call{1} (: true ==> true).  call{2} (: true ==> true).
   while(={j,js} /\ ! uniq js{1}). auto. progress.  auto. rnd{1}. rnd{2}.
-  rnd{1}. auto. progress. apply dcond_ll. apply mu_FD; trivial. apply dpoly_ll. smt(@Bl.FD). smt(). trivial. trivial.   
+  rnd{1}. auto. progress. apply dcond_ll. apply mu_FD; trivial. apply dpoly_ll. smt(@Bl.FD). smt(). trivial. trivial. *)  
 qed.
 
 lemma PolyComPed_Strong_Hiding  &m :
